## Lecture 9

- Use definitions to simplify expressions till no further simplification is possible 
- An “answer” is an expression that cannot be further simplified 
- Built-in simplifications 
- $3+5 -> 8$
- True || False -> True

```haskell
power :: Int -> Int -> Int 
power x 0 = 1 
power x n = x * power x (n-1)
```

Then we have 

```haskell
power 3 2
---> 3 * power 3 (2-1)
---> 3 * power 3 1
---> 3 * 3 *  power 3 (1-1)
---> 3 * 3 *  power 3 0
---> 3 * 3 * 1 
---> 9
```

#### Two ways of computing 

We have

```haskell
(8+3)*(5-3)---> 11*(5-3) ---> 11*2---> 22

(8+3)*(5-3)--->(8+3)*2 ---> 11*2---> 22
```

We also have 

```haskell
power (5+2) (4-4) ---> power (5+2) 0 ---> 1

power (5+2) (4-4) ---> power 7 (4-4) ---> power 7 0 ---> 1
```

#### Lazy Evaluation

We also have 

```haskell
power (3 `div` 0) 0 = 1 
```

- Any Haskell expression is of the form  $f~~e$ 
- $f$ is the outermost function 
- $e$ is the expression to which it is applied

``` haskell
In head (2: reverse [1..5]) 
f is head 
e is 2: reverse [1..5]
```

The argument is not evaluated if the function definition does not force it to be evaluated ---> *Lazy evaluation*

```haskell 
inflist :: [Integer]
inflist = infrom 0 
infrom :: Integer -> [Integer]
infrom n = n: infrom (n+1)

inflist = [0:1:2:3..]
head inflist = head (0: infrom 1) = 0
```

```haskell 
head (2: reverse [1..5])= 2
```

``` haskell
infList = infFrom 0
infFrom n = n: infFrom (n+1)

take 2 infList
---> 0:(take 1 (infrom 1))
---> 0:1: (take 0 (infrom 2))
---> 0:1:[] 
---> [0,1]
```

```haskell
[m..] = [m, m+1, m+2,..]
[m, m+d,..] = [m, m+d, m+2d, m+3d,..]
```

### Higher Order functions
```haskell
capitalize :: String -> String 
capitalize "" = "" 
capitalize (c:cs) = toUpper c: capitalize cs 

sqrList :: [Integer] -> [Integer] 
sqrList [] = [] 
sqrList (x:xs) = x^2 : sqrList xs
```

```haskell
map (+ 3) [2,6,8] = [5,9,11]
map (* 2) [2,6,8] = [4,12,16] 
map (^2) [1,2,3,4] = [1,4,9,16]
```

Given a list of lists, sum the lengths of inner lists

```haskell
sumLength :: [[Int]] -> Int 
sumLength [] = 0 
sumLength (x:xs) = length x + sumLength xs
```

But using Map, we have

```haskell
sumLength l = sum (map length l)
```

###  Map
```haskell
map f [] = [] 
map f (x:xs) = f x: map f xs
```

The type of Map is 

```haskell
map :: (a -> b) -> [a] -> [b]
```

### Filter 
to select all even number from the list

```haskell
allEvens :: [Int] -> [Int] 
allEvens [] = [] 
allEvens (x:xs) 
	| even x = x: allEvens xs 
	| otherwise = allEvens xs

```

But we can also write it as 

```haskell
allEvens l = filter even l  
```

```ad-info
title: Note
 We have certain builtin functions which you should review such as `elem`, `divMod`, `cycle`, `repeat`, etc

```

A generator  p<-l produces a list of candidates 
```haskell
[e | p <- l, Q] = concat (map f l) where f p = [e | Q] f _ = []
```

Built-in function: `concatMap f l = concat $ map f l`

```haskell
[n^2 | n <- [1..7], even n] 
---> concatMap f [1..7] where f n = [n^2 | even n] 
---> concatMap f [1..7] where f n = if even n then [n^2] else [] 
---> concat [[], [4], [], [16], [], [36], []] 
---> [4, 16, 36]
```

```haskell
primes = sieve [2..] where sieve (p:xs) = p:sieve [x | x <- xs, x `mod` p /= 0]
```

## Lecture 10

```haskell

import Data.Char

toupper :: Char -> Char
toupper c = if ord c > 96 then chr ( ord c - 32) else c


toupperword :: [Char] -> [Char]
toupperword []=[]
toupperword (x:y)= ((toupper x) : (toupperword y))
```

### takeWhile and more

``take n l``  returns n-element prefix of list l

```haskell
takeWhile :: (a -> Bool) -> [a] -> [a]
takeWhile (> 7) [8,1,9,10] = [8] 
takeWhile (< 10)[8,1,9,10] = [8,1,9]
```

It takes till the element satisfies and stops when an element does not satisfy.
Similarly, dropWhile

`` position c s`` returns the first position in s where c occurs (or length s)

```haskell
position c s = length (takeWhile (/= c) s)
```

### Zip and ZipWith

``zip`` forms a list of pairs from two lists
``` haskell
zip:: [a]-> [b]-> [(a,b)]
zip [] _ = []
zip _ [] = []
zip [x:xs] [y:ys] = (x,y): zip [xs] [ys]
```

``zipWith`` combines two lists using a function

```haskell
zipWith :: (a -> b -> c)-> [a]->[b]->[c]
zipWith f [] _ = []
zipWith f _ [] = []
zipWith f [x:xs] [y:ys] = f x y: zipWith f [xs] [ys]
```

So we have 
``zipWith (+) [0,2,4,6,8] [1,3,5,7] = [1,5,9,13] ``

### Combining Elements
To find the sum of all numbers in a list
```haskell
sum :: [Int] -> Int
sum []=0
sum [x:xs]= x + sum[xs]
```

Multiply all numbers in a list 

``` haskell
product :: [Int] -> Int
product [] = 1
product (x:xs) = x* product xs
```

Well, Haskell has a built in function to combine. 

### foldr

This function takes a function and a base case as input and then repeats it.

```haskell
foldr :: (a->b->b)->b->[a]->b
foldr f v [] = v
foldr f v (x:xs) = f x (foldr f v xs)
```

Computation:

```haskell
foldr f v [x1, x2, x3]
= f x1 (foldr f v [x2 x3 ])
= f x1 (f x2 (foldr f v [x3]))
= f x1 (f x2 (f x3 (foldr f v [])))
= f x1 (f x2 (f x3 v))
```


So if the list is 
``xs= x1: (x2:(x3:....................)) ``

then 

`` foldr f v xs = x1 `f` (x2 `f`(............. (xn `f` v)))

So we get

```haskell
sum = foldr (+) 0
product = foldr (*) 1
length = foldr f 0 
	where 
		f x n = n+1
```



### Anonymous functions

naming is hard. So we use `\` .

``length = foldr (\ x n -> n+1) 0


```haskell
length [4,5,6] 
= foldr (\ x n -> n+1) 0 [4,5,6] 
= (\ x n -> n+1) 4 (foldr \ x n -> n+1 0 [5,6])
= (\ x n -> n+1) 4 ( (\ x n -> n+1) 5(foldr \ x n -> n+1 0 [6]) )
= (\ x n -> n+1) 4 ( (\ x n -> n+1) 5  ((\ x n -> n+1) 6 (foldr \ x n -> n+1 0 [])))
= (\ x n -> n+1) 4 ( (\ x n -> n+1) 5  ((\ x n -> n+1) 6 0))
=  (\ x n -> n+1) 4 ( (\ x n -> n+1) 5 1)
=   (\ x n -> n+1) 4  2
= 3
```

### More foldr examples

```haskell
foldr f [] [x1, x2, x3]
= f x1 (f x2 (f x3 []))

So we have foldr (:) [] is equivalent to the identity function on lists

concat is just foldr (++) []
```

### foldr1 

Sometimes there is no natural value to assign to the empty list.
For example, finding the maximum value in a list. 
Maximum is undefined for empty list.

```haskell 
foldr1 :: (a->a->a)->[a]->a
foldr1 f [x] = x
foldr1 f (x:xs) = f x (foldr1 f xs)
```
 
so we have ``maximum = foldr1 max``

### foldl 
```haskell
foldl :: (b -> a -> b) -> b -> [a] -> b 
foldl f v [] = v 
foldl f v (x:xs) = foldl f (f v x) xs
```

Example:

Let``f n c = 10* n + digitToInt c``

```haskell
strToNum "234" 
= foldl f 0 "234" 
= foldl f (f 0 '2') "34" 
= foldl f (f (f 0 '2') '3') "4" 
= foldl f (f (f (g 0 '2') '3') '4') "" 
= f (f (f 0 '2') '3') '4' 
= 10 * (f (f 0 '2') '3') + 4 
= 10 * (10 * (f 0 '2') + 3) + 4 
= 10 * (10 * (10*0 + 2) + 3) + 4 
= 234
```
Here the folding is done a bit differently, but opening is sort of same


### Difference between foldl and foldr

- With `foldl` you then place the initial value (here `0`) at the **left-most** position and fill the spaces between the numbers with **left-to-right** arrows.
- With `foldr` you then place the initial value (here `0`) at the **right-most** position and fill the spaces between the numbers with **right-to-left** arrows.

This gives you the following ordering:

- foldl: `0→1→2→3→4`
- foldr: `1←2←3←4←0`

In both cases, in accordance with the direction of the arrows, the initial value (here `0`) comes before the list element that is first viewed.

put brackets around those two numbers that come first (be mindful, _first_ does not mean _left-most_ here). When you then treat this bracketed expression as one single value, you can think of it as always bracketing the first two values. You will then get this:

- foldl: `((((0→1)→2)→3)→4)`
- foldr: `(1←(2←(3←(4←0))))`


``` haskell
foldl f 0 [1,2,3,4] == (f (f (f (f 0 1) 2) 3) 4)
```


```haskell
foldr f 0 [1,2,3,4] == (f 1 (f 2 (f 3 (f 4 0))))
```
## Lecture 11
### foldl'

We know ``foldl`` requires a huge amount of RAM because of Lazy evaluation. We will have huge expressions around. 

So we use the eager version of foldl. 

It is defined in ``Data.List``

```haskell

foldl' :: (b -> a -> b) -> b -> [a] -> b 
foldl' f v [] = v 
foldl' f v (x:xs) = y `seq` foldl' f y xs where y = f v x
```

`seq` evaluates the first argument first and then returns the second argument.

- essentially, `fold'` is nicer but goes against haskell's lazy evaluation 

### flip 
``flip :: (a -> b -> c) -> b -> a -> c``

- swaps the arguments
So we have 

```haskell
flip (:) [1..10] 0 = [0..10]
```




























## Lecture 17

```haskell
revInto xs ys = rev xs ++ ys

revInto [] ys = rev [] ++ ys = ys

revInto (x:xs) ys = rev (x:xs) ++ ys = rev xs ++ [x] ++ ys= rev xs ++ (x:ys)=revInto xs (x:ys)
```

```haskell
fibs

= [fib n| n<-[0..]]

=fib 0: fib 1: [fib n|n <-[2..]]

=0:1:[fib (n-2) + fib (n-1)| n<-[2..]]

=0:1:[fib(n-1)+fib n| n<-[1..]]

=0:1:zipWith (+) [fib (n-1)|n<-[1..]] [fib n| n<-[1..]]

=0:1:zipWith (+) [fib (n)|n<-[0,1..]] [fib n| n<-[1..]]

=0:1:zipWith (+) fibs (tail fibs )

```

